theories/ordinals/MoreAck/fol_Examples.v
@@ -11,12 +11,75 @@ Fail Compute arity LNT (inl LT).
 
 Check var _ 1: Term LNT.
 Check  apply LNT Zero (Tnil _) : Term LNT. 
-About Tcons. 
 
 (* begin snippet v1Plus0 *)
 (** v1 + 0 *)
-Check apply LNN Plus 
-  (Tcons LNN 1 (var _ 1) 
-     (Tcons _ 0 (apply LNN Zero (Tnil _))
-        (Tnil _))).
+Example t1_0: Term LNN :=
+ apply LNN Plus 
+   (Tcons LNN _ (var LNN  1)
+     (Tcons LNN _ (apply LNN Zero (Tnil _)) (Tnil _))). 
 (* end snippet v1Plus0 *)
+
+(* begin snippet instantiations *)
+
+Module InLNN.
+
+Notation Tcons := (Tcons LNN _). 
+Notation Tnil := (Tnil LNN). 
+Notation var := (var LNN).
+Notation apply := (apply LNN). 
+Notation forallNN := (forallH LNN).
+Notation atomicNN := (atomic LNN). 
+Notation impNN := (impH LNN).
+Notation notNN := (notH LNN).
+Notation equal t1 t2 := (equal LNN t1 t2).
+
+Notation orNN := (orH LNN).
+Notation andNN := (andH LNN).
+Notation iffNN := (iffH LNN).
+Notation existNN := (existH LNN).
+
+
+Notation plusNN t1 t2:= (apply Plus (Tcons t1 (Tcons t2 Tnil))).
+Notation ltNN t1 t2 := (atomicNN LT (Tcons t1 (Tcons t2 Tnil))). 
+Notation zeroNN := (apply Zero Tnil).
+Notation succNN t := (apply Succ (Tcons t Tnil)).
+Fixpoint termOfNat n :=
+  match n with 
+    0 => zeroNN
+  | S p => succNN (termOfNat p)
+  end.
+(* end snippet instantiations *)
+
+(* begin snippet v1Plus01 *)
+Example t1: Term LNN := (plusNN (var 1) zeroNN). 
+(* end snippet v1Plus01 *)
+
+
+(** forall v0 v1, v0 < v1 -> v0 < v1 + v0 *)
+(* begin snippet f1Example *)
+Example f1 : Formula LNN :=
+  forallNN 0 
+    (forallNN 1 
+       (impNN 
+          (ltNN (var 0) (var  1))
+          (ltNN (var 0) (plusNN (var 1) (var 0))))).  
+(* end snippet f1Example *)
+
+(* begin snippet f2Example *)
+Example f2 : Formula LNN :=
+  forallNN 0 (existNN 1 (ltNN (var 0) (var 1))).
+(* end snippet f2Example *)
+
+(** depth-order vs structural order *)
+(* begin snippet ltDepth1:: no-out *)
+Goal lt_depth _ 
+  (existNN 1 (ltNN (plusNN (termOfNat 42) (var 3)) (var 1))) f2.
+Proof. red; cbn; auto with arith. Qed. 
+(* end snippet ltDepth1 *)
+End InLNN.
+
+
+
+
+
