theories/ordinals/Ackermann/LNN.v
@@ -40,9 +40,9 @@ Definition Zero : Term := apply LNN Zero (Tnil LNN).
 Definition LT (x y : Term) : Formula :=
   atomic LNN LT (Tcons LNN 1 x (Tcons LNN 0 y (Tnil LNN))). 
 
-Lemma LNN_dec : language_decideable LNN.
+Lemma LNN_dec : language_decidable LNN.
 Proof.
-unfold language_decideable in |- *.
+unfold language_decidable in |- *.
 split; decide equality.
 Qed.
 
